backend/LTL_coop.v
@@ -24,34 +24,39 @@ Inductive LTL_core : Type :=
              (f: function)            (**r function currently executing *)
              (sp: val)                (**r stack pointer *)
              (pc: node)               (**r current program point *)
-             (ls: locset),            (**r location state *)
+             (ls: locset)             (**r location state *)
+             (retty: option typ),     (**r return type at halted *)
       LTL_core
   | LTL_Block:
       forall (stack: list stackframe) (**r call stack *)
              (f: function)            (**r function currently executing *)
              (sp: val)                (**r stack pointer *)
              (bb: bblock)             (**r current basic block *)
-             (ls: locset),            (**r location state *)
+             (ls: locset)             (**r location state *)
+             (retty: option typ),     (**r return type at halted *)
       LTL_core
   | LTL_Callstate:
       forall (stack: list stackframe) (**r call stack *)
              (f: fundef)              (**r function to call *)
-             (ls: locset),            (**r location state of caller *)
+             (ls: locset)             (**r location state of caller *)
+             (retty: option typ),     (**r return type at halted *)
       LTL_core
   | LTL_Returnstate:
       forall (stack: list stackframe) (**r call stack *)
              (retty: option typ)      (**r optional return register int-floatness *)
-             (ls: locset),            (**r location state of callee *)
+             (ls: locset)             (**r location state of callee *)
+             (retty: option typ),     (**r return type at halted *)
       LTL_core.
 
 Section LTL_COOP.
 Variable hf : I64Helpers.helper_functions.
 
-Definition LTL_at_external (c: LTL_core) : option (external_function * signature * list val) :=
+Definition LTL_at_external (c: LTL_core) 
+  : option (external_function * signature * list val) :=
   match c with
-    | LTL_State _ _ _ _ _ => None
-    | LTL_Block _ _ _ _ _ => None
-    | LTL_Callstate s f rs => 
+    | LTL_State _ _ _ _ _ _ => None
+    | LTL_Block _ _ _ _ _ _ => None
+    | LTL_Callstate s f rs retty => 
       match f with
         | Internal f => None
         | External ef => 
@@ -60,116 +65,116 @@ Definition LTL_at_external (c: LTL_core) : option (external_function * signature
                                      (map rs (loc_arguments (ef_sig ef))))
            else None
       end
-    | LTL_Returnstate _ _ _ => None
+    | LTL_Returnstate _ _ _ _ => None
  end.
 
 Definition LTL_after_external (vret: option val) (c: LTL_core) : option LTL_core :=
   match c with 
-    | LTL_Callstate s f rs => 
+    | LTL_Callstate s f rs retty => 
       match f with
         | Internal f => None
         | External ef => 
           match vret with
             | None => Some (LTL_Returnstate s (sig_res (ef_sig ef))
                 (Locmap.setlist (map R (loc_result (ef_sig ef))) 
-                  (encode_long (sig_res (ef_sig ef)) Vundef) rs))
+                  (encode_long (sig_res (ef_sig ef)) Vundef) rs) retty)
             | Some v => Some (LTL_Returnstate s (sig_res (ef_sig ef))
                 (Locmap.setlist (map R (loc_result (ef_sig ef))) 
-                  (encode_long (sig_res (ef_sig ef)) v) rs))
+                  (encode_long (sig_res (ef_sig ef)) v) rs) retty) 
           end
       end
     | _ => None
   end.
 
 Inductive ltl_corestep (ge:genv): LTL_core -> mem -> LTL_core -> mem -> Prop :=
-  | ltl_exec_start_block: forall s f sp pc rs m bb,
+  | ltl_exec_start_block: forall s f sp pc rs m bb retty,
       (fn_code f)!pc = Some bb ->
-      ltl_corestep ge (LTL_State s f sp pc rs) m
-        (LTL_Block s f sp bb rs) m
-  | ltl_exec_Lop: forall s f sp op args res bb rs m v rs',
+      ltl_corestep ge (LTL_State s f sp pc rs retty) m
+        (LTL_Block s f sp bb rs retty) m
+  | ltl_exec_Lop: forall s f sp op args res bb rs m v rs' retty,
       eval_operation ge sp op (reglist rs args) m = Some v ->
       rs' = Locmap.set (R res) v (undef_regs (destroyed_by_op op) rs) ->
-      ltl_corestep ge (LTL_Block s f sp (Lop op args res :: bb) rs) m
-        (LTL_Block s f sp bb rs') m
-  | ltl_exec_Lload: forall s f sp chunk addr args dst bb rs m a v rs',
+      ltl_corestep ge (LTL_Block s f sp (Lop op args res :: bb) rs retty) m
+        (LTL_Block s f sp bb rs' retty) m
+  | ltl_exec_Lload: forall s f sp chunk addr args dst bb rs m a v rs' retty,
       eval_addressing ge sp addr (reglist rs args) = Some a ->
       Mem.loadv chunk m a = Some v ->
       rs' = Locmap.set (R dst) v (undef_regs (destroyed_by_load chunk addr) rs) ->
-      ltl_corestep ge (LTL_Block s f sp (Lload chunk addr args dst :: bb) rs) m
-        (LTL_Block s f sp bb rs') m
-  | ltl_exec_Lgetstack: forall s f sp sl ofs ty dst bb rs m rs',
+      ltl_corestep ge (LTL_Block s f sp (Lload chunk addr args dst :: bb) rs retty) m
+        (LTL_Block s f sp bb rs' retty) m
+  | ltl_exec_Lgetstack: forall s f sp sl ofs ty dst bb rs m rs' retty,
       rs' = Locmap.set (R dst) (rs (S sl ofs ty)) (undef_regs (destroyed_by_getstack sl) rs) ->
-      ltl_corestep ge (LTL_Block s f sp (Lgetstack sl ofs ty dst :: bb) rs) m
-        (LTL_Block s f sp bb rs') m
-  | ltl_exec_Lsetstack: forall s f sp src sl ofs ty bb rs m rs',
+      ltl_corestep ge (LTL_Block s f sp (Lgetstack sl ofs ty dst :: bb) rs retty) m
+        (LTL_Block s f sp bb rs' retty) m
+  | ltl_exec_Lsetstack: forall s f sp src sl ofs ty bb rs m rs' retty,
       rs' = Locmap.set (S sl ofs ty) (rs (R src)) (undef_regs (destroyed_by_setstack ty) rs) ->
-      ltl_corestep ge (LTL_Block s f sp (Lsetstack src sl ofs ty :: bb) rs) m
-        (LTL_Block s f sp bb rs') m
-  | ltl_exec_Lstore: forall s f sp chunk addr args src bb rs m a rs' m',
+      ltl_corestep ge (LTL_Block s f sp (Lsetstack src sl ofs ty :: bb) rs retty) m
+        (LTL_Block s f sp bb rs' retty) m
+  | ltl_exec_Lstore: forall s f sp chunk addr args src bb rs m a rs' m' retty,
       eval_addressing ge sp addr (reglist rs args) = Some a ->
       Mem.storev chunk m a (rs (R src)) = Some m' ->
       rs' = undef_regs (destroyed_by_store chunk addr) rs ->
-      ltl_corestep ge (LTL_Block s f sp (Lstore chunk addr args src :: bb) rs) m
-        (LTL_Block s f sp bb rs') m'
-  | ltl_exec_Lcall: forall s f sp sig ros bb rs m fd,
+      ltl_corestep ge (LTL_Block s f sp (Lstore chunk addr args src :: bb) rs retty) m
+        (LTL_Block s f sp bb rs' retty) m'
+  | ltl_exec_Lcall: forall s f sp sig ros bb rs m fd retty,
       find_function ge ros rs = Some fd ->
       funsig fd = sig ->
-      ltl_corestep ge (LTL_Block s f sp (Lcall sig ros :: bb) rs) m
-        (LTL_Callstate (Stackframe f sp rs bb :: s) fd rs) m
-  | ltl_exec_Ltailcall: forall s f sp sig ros bb rs m fd rs' m',
+      ltl_corestep ge (LTL_Block s f sp (Lcall sig ros :: bb) rs retty) m
+        (LTL_Callstate (Stackframe f sp rs bb :: s) fd rs retty) m
+  | ltl_exec_Ltailcall: forall s f sp sig ros bb rs m fd rs' m' retty,
       rs' = return_regs (parent_locset s) rs ->
       find_function ge ros rs' = Some fd ->
       funsig fd = sig ->
       Mem.free m sp 0 f.(fn_stacksize) = Some m' ->
-      ltl_corestep ge (LTL_Block s f (Vptr sp Int.zero) (Ltailcall sig ros :: bb) rs) m
-        (LTL_Callstate s fd rs') m'
-  | ltl_exec_Lbuiltin: forall s f sp ef args res bb rs m t vl rs' m',
+      ltl_corestep ge (LTL_Block s f (Vptr sp Int.zero) (Ltailcall sig ros :: bb) rs retty) m
+        (LTL_Callstate s fd rs' retty) m'
+  | ltl_exec_Lbuiltin: forall s f sp ef args res bb rs m t vl rs' m' retty,
       external_call' ef ge (reglist rs args) m t vl m' ->
       ~ observableEF hf ef ->
       rs' = Locmap.setlist (map R res) vl (undef_regs (destroyed_by_builtin ef) rs) ->
-      ltl_corestep ge (LTL_Block s f sp (Lbuiltin ef args res :: bb) rs) m
-         (LTL_Block s f sp bb rs') m'
+      ltl_corestep ge (LTL_Block s f sp (Lbuiltin ef args res :: bb) rs retty) m
+         (LTL_Block s f sp bb rs' retty) m'
 (* WE DON'T SUPPORT ANNOT YET
   | ltl_exec_Lannot: forall s f sp ef args bb rs m t vl m',
       external_call' ef ge (map rs args) m t vl m' ->
       ltl_corestep (LTL_Block s f sp (Lannot ef args :: bb) rs) m
          (LTL_Block s f sp bb rs) m' *)
-  | ltl_exec_Lbranch: forall s f sp pc bb rs m,
-      ltl_corestep ge (LTL_Block s f sp (Lbranch pc :: bb) rs) m
-        (LTL_State s f sp pc rs) m
-  | ltl_exec_Lcond: forall s f sp cond args pc1 pc2 bb rs b pc rs' m,
+  | ltl_exec_Lbranch: forall s f sp pc bb rs m retty,
+      ltl_corestep ge (LTL_Block s f sp (Lbranch pc :: bb) rs retty) m
+        (LTL_State s f sp pc rs retty) m
+  | ltl_exec_Lcond: forall s f sp cond args pc1 pc2 bb rs b pc rs' m retty,
       eval_condition cond (reglist rs args) m = Some b ->
       pc = (if b then pc1 else pc2) ->
       rs' = undef_regs (destroyed_by_cond cond) rs ->
-      ltl_corestep ge (LTL_Block s f sp (Lcond cond args pc1 pc2 :: bb) rs) m
-        (LTL_State s f sp pc rs') m
-  | ltl_exec_Ljumptable: forall s f sp arg tbl bb rs m n pc rs',
+      ltl_corestep ge (LTL_Block s f sp (Lcond cond args pc1 pc2 :: bb) rs retty) m
+        (LTL_State s f sp pc rs' retty) m
+  | ltl_exec_Ljumptable: forall s f sp arg tbl bb rs m n pc rs' retty,
       rs (R arg) = Vint n ->
       list_nth_z tbl (Int.unsigned n) = Some pc ->
       rs' = undef_regs (destroyed_by_jumptable) rs ->
-      ltl_corestep ge (LTL_Block s f sp (Ljumptable arg tbl :: bb) rs) m
-        (LTL_State s f sp pc rs') m
-  | ltl_exec_Lreturn: forall s f sp bb rs m m',
+      ltl_corestep ge (LTL_Block s f sp (Ljumptable arg tbl :: bb) rs retty) m
+        (LTL_State s f sp pc rs' retty) m
+  | ltl_exec_Lreturn: forall s f sp bb rs m m' retty,
       Mem.free m sp 0 f.(fn_stacksize) = Some m' ->
-      ltl_corestep ge (LTL_Block s f (Vptr sp Int.zero) (Lreturn :: bb) rs) m
-        (LTL_Returnstate s (sig_res (fn_sig f)) (return_regs (parent_locset s) rs)) m'
-  | ltl_exec_function_internal: forall s f rs m m' sp rs',
+      ltl_corestep ge (LTL_Block s f (Vptr sp Int.zero) (Lreturn :: bb) rs retty) m
+        (LTL_Returnstate s (sig_res (fn_sig f)) (return_regs (parent_locset s) rs) retty) m'
+  | ltl_exec_function_internal: forall s f rs m m' sp rs' retty,
       Mem.alloc m 0 f.(fn_stacksize) = (m', sp) ->
       rs' = undef_regs destroyed_at_function_entry (call_regs rs) ->
-      ltl_corestep ge (LTL_Callstate s (Internal f) rs) m
-        (LTL_State s f (Vptr sp Int.zero) f.(fn_entrypoint) rs') m'
+      ltl_corestep ge (LTL_Callstate s (Internal f) rs retty) m
+        (LTL_State s f (Vptr sp Int.zero) f.(fn_entrypoint) rs' retty) m'
 
-  | ltl_exec_function_external: forall s ef t args res rs m rs' m'
+  | ltl_exec_function_external: forall s ef t args res rs m rs' m' retty
       (OBS: EFisHelper hf ef),
       args = map rs (loc_arguments (ef_sig ef)) ->
       external_call' ef ge args m t res m' ->
       rs' = Locmap.setlist (map R (loc_result (ef_sig ef))) res rs ->
-      ltl_corestep ge (LTL_Callstate s (External ef) rs) m
-          (LTL_Returnstate s (sig_res (ef_sig ef)) rs') m'
+      ltl_corestep ge (LTL_Callstate s (External ef) rs retty) m
+          (LTL_Returnstate s (sig_res (ef_sig ef)) rs' retty) m'
 
-  | ltl_exec_return: forall f sp rs1 bb s retty rs m,
-      ltl_corestep ge (LTL_Returnstate (Stackframe f sp rs1 bb :: s) retty rs) m
-        (LTL_Block s f sp bb rs) m.
+  | ltl_exec_return: forall f sp rs1 bb s retty rs m retty0,
+      ltl_corestep ge (LTL_Returnstate (Stackframe f sp rs1 bb :: s) retty rs retty0) m
+        (LTL_Block s f sp bb rs retty0) m.
 
 Lemma LTL_corestep_not_at_external ge m q m' q':
       ltl_corestep ge q m q' m' -> LTL_at_external q = None.
@@ -181,7 +186,7 @@ Qed.
 Definition LTL_halted (q : LTL_core): option val :=
     match q with 
       (*Return Tlong, which must be decoded*)
-      | LTL_Returnstate nil (Some Tlong) rs => 
+      | LTL_Returnstate nil _ rs (Some Tlong) => 
            match loc_result (mksignature nil (Some Tlong)) with
              | nil => None
              | r1 :: r2 :: nil => 
@@ -193,7 +198,7 @@ Definition LTL_halted (q : LTL_core): option val :=
            end
 
       (*Return a value of any other typ*)
-      | LTL_Returnstate nil (Some retty) rs => 
+      | LTL_Returnstate nil _ rs (Some retty) =>
            match loc_result (mksignature nil (Some retty)) with
             | nil => None
             | r :: TL => match TL with 
@@ -203,7 +208,7 @@ Definition LTL_halted (q : LTL_core): option val :=
            end
 
       (*Return Tvoid - modeled as integer return*)
-      | LTL_Returnstate nil None rs => Some (rs (R AX))
+      | LTL_Returnstate nil _ rs None => Some (rs (R AX))
 
       | _ => None
     end.
@@ -256,7 +261,8 @@ Definition LTL_initial_core (ge:genv) (v: val) (args:list val): option LTL_core 
                                       (Locmap.setlist
                                           (loc_arguments (funsig f)) 
                                           (encode_longs tyl args)
-                                          (Locmap.init Vundef)))
+                                          (Locmap.init Vundef))
+                                      (sig_res (funsig f)))
                      else None
                    | External _ => None
                    end
